Weidenbach_Book/IsaSAT_LLVM.thy
@@ -412,7 +412,11 @@ experiment
 begin
   lemmas [llvm_code] = llvm_version_def
 
-  declare NORMAL_PHASE_def[llvm_inline] DEFAULT_INIT_PHASE_def[llvm_inline] QUIET_PHASE_def[llvm_inline]
+  lemmas [llvm_inline] =
+    unit_propagation_inner_loop_body_wl_fast_heur_code_def
+    NORMAL_PHASE_def DEFAULT_INIT_PHASE_def QUIET_PHASE_def
+    find_unwatched_wl_st_heur_fast_code_def
+
   export_llvm IsaSAT_code_wrapped llvm_version default_opts_impl IsaSAT_code file "code/isasat_restart.ll"
 
 end
